Replacing ExtLib's Show by Ceres's Serializable

src/coq/AstLib.v
@@ -9,8 +9,9 @@
  ---------------------------------------------------------------------------- *)
 
 
-Require Import ZArith.ZArith List.
-Require Import String Omega.
+From Coq Require Import
+     ZArith.ZArith List
+     String Omega.
 Require Import Vellvm.LLVMAst Vellvm.Util.
 Require Import Equalities OrderedType OrderedTypeEx Compare_dec.
 Require Import ExtLib.Core.RelDec ExtLib.Data.Z.
@@ -481,218 +482,204 @@ End ExpInd.
 
 
 (* Display *)
-Require Import ExtLib.Programming.Show.
+Require Import Ceres.Ceres.
 
 Section hiding_notation.
-  Import ShowNotation.
-  Local Open Scope show_scope.
+  Local Open Scope sexp_scope.
 
-  Global Instance show_option {T} `{Show T}: Show (option T) :=
-    { show mt := match mt with
-                 | None => show "None"
-                 | Some t => show "Some " << show t
-                 end }.
+  Global Instance serialize_option {T} `{Serialize T}: Serialize (option T) :=
+    fun mt => match mt with
+           | None => Raw "None"
+           | Some t => [Raw "Some " ; to_sexp t]
+           end.
 
-  Global Instance show_raw_id : Show raw_id :=
-    { show r :=
-        match r with
-        | Name s => s
-        | Anon n => show n
-        | Raw  n => "_RAW_" << show n
-        end
-    }.
+  Global Instance serialize_raw_id : Serialize raw_id :=
+    fun r =>
+      match r with
+      | Name s => Raw s
+      | Anon n => to_sexp n
+      | LLVMAst.Raw  n => [Raw "_RAW_" ; to_sexp n]
+      end.
 
-  Global Instance show_ident : Show ident :=
-    { show id :=
-        match id with
-        | ID_Global r => "@" << show r
-        | ID_Local  r => "%" << show r
-        end
-    }.
+  Global Instance serialize_ident : Serialize ident :=
+    fun id =>
+      match id with
+      | ID_Global r => [Raw "@" ; to_sexp r]
+      | ID_Local  r => [Raw "%" ; to_sexp r]
+      end.
 
-  Global Instance show_instr_id : Show instr_id :=
-    { show ins :=
-        match ins with
-        | IId id => show id
-        | IVoid n => "void<" << show n << ">"
-        end
-    }.
+  Global Instance serialize_instr_id : Serialize instr_id :=
+    fun ins =>
+      match ins with
+      | IId id => to_sexp id
+      | IVoid n => [Raw "void<" ; to_sexp n ; Raw ">"]
+      end.
 
+  Global Instance serialize_ibinop : Serialize ibinop :=
+    fun binop =>
+      match binop with
+      | Add nuw nsw => Raw "add"
+      | Sub nuw nsw => Raw "sub"
+      | Mul nuw nsw => Raw "mul"
+      | Shl nuw nsw => Raw "shl"
+      | UDiv flag => Raw "udiv"
+      | SDiv flag => Raw "sdiv"
+      | LShr flag => Raw "lshr"
+      | AShr flag => Raw "ashr"
+      | URem | SRem => Raw "rem"
+      | And => Raw "and"
+      | Or => Raw "or"
+      | Xor => Raw "xor"
+      end.
 
-  Global Instance show_ibinop : Show ibinop :=
-    { show binop :=
-        match binop with
-        | Add nuw nsw => "add"
-        | Sub nuw nsw => "sub"
-        | Mul nuw nsw => "mul"
-        | Shl nuw nsw => "shl"
-        | UDiv flag => "udiv"
-        | SDiv flag => "sdiv"
-        | LShr flag => "lshr"
-        | AShr flag => "ashr"
-        | URem | SRem => "rem"
-        | And => "and"
-        | Or => "or"
-        | Xor => "xor"
-        end
-    }.
+  Global Instance serialize_fbinop : Serialize fbinop :=
+    fun fbinop =>
+      match fbinop with
+      | FAdd => Raw "fadd"
+      | FSub => Raw "fsub"
+      | FMul => Raw "fmul"
+      | FDiv => Raw "fdiv"
+      | FRem => Raw "frem"
+      end.
 
-  Global Instance show_fbinop : Show fbinop :=
-    { show fbinop :=
-        match fbinop with
-        | FAdd => "fadd"
-        | FSub => "fsub"
-        | FMul => "fmul"
-        | FDiv => "fdiv"
-        | FRem => "frem"
-        end
-    }.
+  Global Instance serialize_icmp : Serialize icmp :=
+    fun cmp =>
+      [Raw "icmp " ;
+         match cmp with
+         | Eq => Raw "eq"
+         | Ne => Raw "ne"
+         | Ugt => Raw "ugt"
+         | Uge => Raw "uge"
+         | Ult => Raw "ult"
+         | Ule => Raw "ule"
+         | Sgt => Raw "sgt"
+         | Sge => Raw "sge"
+         | Slt => Raw "slt"
+         | Sle => Raw "sle"
+         end].
 
-  Global Instance show_icmp : Show icmp :=
-    { show cmp :=
-        "icmp " <<
-                match cmp with
-                | Eq => "eq"
-                | Ne => "ne"
-                | Ugt => "ugt"
-                | Uge => "uge"
-                | Ult => "ult"
-                | Ule => "ule"
-                | Sgt => "sgt"
-                | Sge => "sge"
-                | Slt => "slt"
-                | Sle => "sle"
-                end
-    }.
+  Global Instance serialize_fcmp : Serialize fcmp :=
+    fun cmp =>
+      [Raw "fcmp " ;
+         match cmp with
+           FFalse => Raw "ffalse"
+         | FOeq => Raw "foeq"
+         | FOgt => Raw "fogt"
+         | FOge => Raw "foge"
+         | FOlt => Raw "folt"
+         | FOle => Raw "fole"
+         | FOne => Raw "fone"
+         | FOrd => Raw "ford"
+         | FUno => Raw "funo"
+         | FUeq => Raw "fueq"
+         | FUgt => Raw "fugt"
+         | FUge => Raw "fuge"
+         | FUlt => Raw "fult"
+         | FUle => Raw "fule"
+         | FUne => Raw "fune"
+         | FTrue => Raw "ftrue"
+         end].
 
-  Global Instance show_fcmp : Show fcmp :=
-    { show cmp :=
-        "fcmp " <<
-                match cmp with
-                  FFalse => "ffalse"
-                | FOeq => "foeq"
-                | FOgt => "fogt"
-                | FOge => "foge"
-                | FOlt => "folt"
-                | FOle => "fole"
-                | FOne => "fone"
-                | FOrd => "ford"
-                | FUno => "funo"
-                | FUeq => "fueq"
-                | FUgt => "fugt"
-                | FUge => "fuge"
-                | FUlt => "fult"
-                | FUle => "fule"
-                | FUne => "fune"
-                | FTrue => "ftrue"
-               end
-    }.
-
-  Fixpoint show_typ' typ :=
+  Fixpoint serialize_typ' typ :=
     match typ with
-    | TYPE_I sz => ("i" << show sz)
-    | TYPE_Pointer t => ((show_typ' t) << "*")%string
-    | _ => "(show_typ todo)"
+    | TYPE_I sz => [Raw "i" ; to_sexp sz]
+    | TYPE_Pointer t => [serialize_typ' t ; Raw "*"]
+    | _ => Raw "(show_typ todo)"
     end.
 
-  Global Instance show_typ : Show typ := show_typ'.
+  Global Instance serialize_typ : Serialize typ := serialize_typ'.
 
-  Section WithShowT.
+  Section WithSerializeT.
     Variable (T:Set).
-    Context `{showT : Show T}.
+    Context `{serializeT : Serialize T}.
 
-  Fixpoint show_exp' (v : exp T) :=
-    match v with
-    | EXP_Ident id => show id
-    | EXP_Integer x => show x
-    | EXP_Bool b => show b
-    | EXP_Null => "null"
-    | EXP_Zero_initializer => "zero initializer"
-    | EXP_Cstring s => s
-    | EXP_Undef => "undef"
-    | OP_IBinop iop t v1 v2 =>
-      ((show iop) << " " << (show t)
-                  << " " << (show_exp' v1)
-                  << " " << (show_exp' v2))%string
-    | OP_ICmp cmp t v1 v2 =>
-      ((show cmp) << " " << (show t)
-                  << " " << (show_exp' v1)
-                  << " " << (show_exp' v2))%string
-    | OP_GetElementPtr t ptrval idxs =>
-      "getelementptr"
-    | _ => "show_exp todo"
-    end.
+    Fixpoint serialize_exp' (v : exp T) :=
+      match v with
+      | EXP_Ident id => to_sexp id
+      | EXP_Integer x => to_sexp x
+      | EXP_Bool b => to_sexp b
+      | EXP_Null => Raw "null"
+      | EXP_Zero_initializer => Raw "zero initializer"
+      | EXP_Cstring s => Raw s
+      | EXP_Undef => Raw "undef"
+      | OP_IBinop iop t v1 v2 =>
+        [to_sexp iop ; Raw " " ; to_sexp t
+                    ; Raw " " ; serialize_exp' v1
+                    ; Raw " " ; serialize_exp' v2]
+      | OP_ICmp cmp t v1 v2 =>
+        [to_sexp cmp ; Raw " " ; to_sexp t
+                    ; Raw " " ; serialize_exp' v1
+                    ; Raw " " ; serialize_exp' v2]
+      | OP_GetElementPtr t ptrval idxs =>
+        Raw "getelementptr"
+      | _ => Raw "to_sexp_exp todo"
+      end.
 
-  Global Instance show_exp : Show (exp T) := show_exp'.
+    Global Instance serialize_exp : Serialize (exp T) := serialize_exp'.
+    Global Instance serialize_int : Serialize int := Serialize_Integral Integral_Z.
 
-  Global Instance show_int : Show int := Show_Z.
+    Global Instance serialize_texp : Serialize (texp T) :=
+      fun '(t, e) =>
+          [to_sexp t ; Raw " " ; to_sexp e ].
 
-  Global Instance show_texp : Show (texp T) :=
-    { show '(t, e) :=
-        show t << " " << show e }.
-
-  Definition show_opt {A:Type} `{AS:Show A} (s:string) : Show (option A) :=
-    fun x =>
+    Definition serialize_opt {A:Type} `{AS:Serialize A} (s:string) : Serialize (option A) :=
+      fun x =>
         match x with
-        | None => empty
-        | Some a => s << show a
+        | None => Raw ""
+        | Some a => [Raw s ; to_sexp a]
         end.
 
-  Global Instance show_instr : Show (instr T) :=
-    { show instr :=
+    Global Instance serialize_instr : Serialize (instr T) :=
+      fun instr =>
         match instr with
-        | INSTR_Op op => show op
+        | INSTR_Op op => to_sexp op
 
         | INSTR_Load vol t ptr align =>
-          "load " << (show t) << " " << (show ptr)
-                   << (@show_opt _ show_int ", align " align)
+          [Raw "load " ; to_sexp t ; Raw " " ; to_sexp ptr
+           ; @serialize_opt _ serialize_int ", align " align]
 
         | INSTR_Store vol tval ptr align =>
-          ("store " << (show tval) << " " << (show ptr)
-                    << (@show_opt _ show_int ", align " align))%string
+          [Raw "store " ; to_sexp tval ; Raw " " ; to_sexp ptr
+           ; @serialize_opt _ serialize_int ", align " align]
 
         | INSTR_Alloca t nb align =>
-          ("alloca " << (show t) << (@show_opt _ show_int ", align " align))%string
+          [Raw "alloca " ; to_sexp t ; @serialize_opt _ serialize_int ", align " align]
         (*
            | INSTR_Call
            | INSTR_Phi
            | INSTR_Alloca
          *)
-        | _ => "string_of_instr todo"
-        end
-    }.
+        | _ => Raw "string_of_instr todo"
+        end.
 
-  Global Instance show_terminator : Show (terminator T) :=
-    { show t :=
+    Global Instance serialize_terminator : Serialize (terminator T) :=
+      fun t =>
         match t with
-        | TERM_Ret v => "ret " << (show v)
-        | TERM_Ret_void => "ret"
-        | _ => "string_of_terminator todo"
-        end
-    }.
+        | TERM_Ret v => [Raw "ret " ; to_sexp v]
+        | TERM_Ret_void => Raw "ret"
+        | _ => Raw "string_of_terminator todo"
+        end.
 
-  Global Instance show_instr_id_instr : Show (instr_id * (instr T)) :=
-    { show '(iid, i) := show iid << " = " << show i }.
+    Global Instance serialize_instr_id_instr : Serialize (instr_id * (instr T)) :=
+      fun '(iid, i) => [to_sexp iid ; Raw " = " ; to_sexp i].
 
-  Global Instance show_block : Show (block T) :=
-    { show block :=
-        ("Block "
-           << show (blk_id T block) << ": " )
-           << iter_show (List.map show (blk_code T block))
-    }.
+    Global Instance serialize_block : Serialize (block T) :=
+      fun block =>
+        [Raw "Block "
+         ; to_sexp (blk_id T block) ; Raw ": " ;
+           to_sexp (blk_code T block)].
 
-  Global Instance show_definition_list_block : Show (definition T (list (block T))) :=
-    { show defn := ("defn: " << iter_show (List.map show (df_instrs T _ defn))) }.
+    Global Instance serialize_definition_list_block : Serialize (definition T (list (block T))) :=
+      fun defn => [Raw "defn: " ; to_sexp (df_instrs T _ defn)].
 
-  Global Instance show_tle_list_block : Show (toplevel_entity T (list (block T))) :=
-   { show tle :=
-       match tle with
-       | TLE_Definition defn => show defn
-       | _ => "string_of_tle_list_block todo"
-       end
-   }.
+    Global Instance serialize_tle_list_block : Serialize (toplevel_entity T (list (block T))) :=
+      fun tle =>
+        match tle with
+        | TLE_Definition defn => to_sexp defn
+        | _ => Raw "string_of_tle_list_block todo"
+        end.
 
-  End WithShowT.
+  End WithSerializeT.
 End hiding_notation.
 
 Section WithType.
