src/coq/Denotation.v
@@ -16,7 +16,6 @@ From Coq Require Import
 Require Import Integers Floats.
 
 From ExtLib Require Import
-     Programming.Show
      Structures.Monads
      Structures.Functor
      Eqv.
@@ -38,6 +37,8 @@ From Vellvm Require Import
      TypeUtil
      Handlers.Intrinsics.
 
+Require Import Ceres.Ceres.
+
 (* YZ: Undesirable dependency on Handlers/Intrinsics: move [intrinsic_exp] somewhere else? *)
 
 Import Sum.
@@ -45,7 +46,6 @@ Import Subevent.
 Import EqvNotation.
 Import ListNotations.
 Import MonadNotation.
-Import ShowNotation.
 
 Set Implicit Arguments.
 Set Contextual Implicit.
@@ -388,7 +388,7 @@ Module Denotation(A:MemoryAddress.ADDRESS)(LLVMEvents:LLVM_INTERACTIONS(A)).
            (top:option dtyp) (o:exp dtyp) {struct o} : itree exp_E uvalue :=
         let eval_texp '(dt,ex) := denote_exp (Some dt) ex
         in
-        (* debug ("Evaluating expression " ++ to_string o);; *)
+        debug ("Evaluating expression " ++ to_string o);;
         match o with
         | EXP_Ident i =>
           translate lookup_E_to_exp_E (lookup_id i)
@@ -909,196 +909,3 @@ Module Denotation(A:MemoryAddress.ADDRESS)(LLVMEvents:LLVM_INTERACTIONS(A)).
                 ) _ (Call dt f_value args).
 End Denotation.
 
-  (****************************** SCRAPYARD ******************************)
-
-  (* Code related to environment unused for global env that are static.
-     Should be reused to handle locals.
-   *)
-(*
-Definition env  := ENV.t dvalue.
-
-Definition env_of_assoc {A} (l:list (raw_id * A)) : ENV.t A :=
-  List.fold_left (fun e '(k,v) => ENV.add k v e) l (@ENV.empty A).
-
-
-  Fixpoint string_of_env' (e:list (raw_id * dvalue)) :=
-    match e with
-    | [] => empty
-    | (lid, _)::rest => ((to_string lid) << " " << (string_of_env' rest))%show
-    end.
-
-  Instance show_env : Show env := fun env => string_of_env' (ENV.elements env).
-  Definition add_env := ENV.add.
-*)
-  (* Code related to the previous structure of states.
-     Will likely not be reused as is. The structure of states should now be
-     defined by successive states monads introduced by sucessive handlers.
-   *)
-(*
-  Inductive frame : Type :=
-  | KRet      (e:env) (id:local_id) (q:pc)
-  | KRet_void (e:env) (p:pc)
-  .
-  Definition stack := list frame.
-
-  Definition state := (genv * pc * env * stack)%type.
-
-  Definition pc_of (s:state) :=
-    let '(g, p, e, k) := s in p.
-
-  Definition env_of (s:state) :=
-    let '(g, p, e, k) := s in e.
-
-  Definition stack_of (s:state) :=
-    let '(g, p, e, k) := s in k.
-*)
-
-  (* Code related to manipulating the stack frame during a return *)
-  (* Should be mostly irrelevant, but needs to be pondered. *)
-  (* The local env aspect should be handled by interpreting Locals into
-   a stack of environment. The ret terminator introduces a special pop
-   event when denoted.
-   The id part, hosting the returned value, should be handled by being given
-   to the denotation of the Call instruction: it is a call event, expected a
-   dvalue, followed by the appropriate store event.
-   The program counter part should be irrelevant in this style of semantics.
-   *)
-
-    (* match k with *)
-    (* | [] => halt dv        *)
-    (* | (KRet e' id p') :: k' => cont (g, p', add_env id dv e', k') *)
-    (* | _ => raise_p pc "IMPOSSIBLE: Ret op in non-return configuration"  *)
-    (* end *)
-
-  (* match k with *)
-    (* | [] => halt DVALUE_None *)
-    (* | (KRet_void e' p')::k' => cont (g, p', e', k') *)
-    (* | _ => raise_p pc "IMPOSSIBLE: Ret void in non-return configuration" *)
-    (* end *)
-
-
-(* Defining the Global Environment ------------------------------------------------------- *)
-(*
-
-*)
-(* Assumes that the entry-point function is named "fname" and that it takes
-   no parameters *)
-
-(* COMMENTING OUT
-Definition init_state (fname:string) : itree (failureE +' debugE) state :=
-  g <- build_global_environment ;;
-  fentry <- trywith ("INIT: no function named " ++ fname) (find_function_entry CFG (Name fname)) ;;
-  let 'FunctionEntry ids pc_f := fentry in
-    ret (g, pc_f, (@ENV.empty dvalue), []).
-
-CoFixpoint step_sem (r:result) : itree (failureE +' debugE) dvalue :=
-  match r with
-  | Done v => ret v
-  | Step s => x <- step s ;; ITreeDefinition.Tau (step_sem x)
-  end.
-
-(* TODO: move elsewhere? *)
-Fixpoint combine_lists_err {A B:Type} (l1:list A) (l2:list B) : err (list (A * B)) :=
-  match l1, l2 with
-  | [], [] => ret []
-  | x::xs, y::ys =>
-    l <- combine_lists_err xs ys ;;
-    ret ((x,y)::l)
-  | _, _ => failwith "combine_lists_err: different lenth lists"
-  end.
-
-END OF COMMENTING OUT *)
-(*
-YZ : Should not be used anymore?
-Inductive result :=
-| Done (v:dvalue)
-| Step (s:state)
-.
-
-Definition raise_p {X} (p:pc) s : itree (failureE +' debugE) X := raise (s ++ " in block: " ++ (to_string p)).
-Definition cont (s:state)  : itree (failureE +' debugE) result := ret (Step s).
-Definition halt (v:dvalue) : itree (failureE +' debugE) result := ret (Done v).
-
- *)
-(*
-Definition jump (fid:function_id) (bid_src:block_id) (bid_tgt:block_id) (g:genv) (e_init:env) (k:stack) : itree (failureE +' debugE) result :=
-  let eval_phi (e:env) '(iid, Phi t ls) :=
-      match assoc RawIDOrd.eq_dec bid_src ls with
-      | Some op =>
-        let dt := eval_typ t in
-        dv <- denote_exp g (Some dt) op ;;
-        ret (add_env iid dv e)
-      | None => raise ("jump: phi node doesn't include block " ++ to_string bid_src )
-      end
-  in
-  debug ("jumping to: " ++ to_string bid_tgt) ;;
-  match find_block_entry CFG fid bid_tgt with
-  | None => raise ("jump: target block " ++ to_string bid_tgt ++ " not found")
-  | Some (BlockEntry phis pc_entry) =>
-      e_out <- monad_fold_right eval_phi phis e_init ;;
-      cont (g, pc_entry, e_out, k)
-  end.
- *)
-
-    (* YZ: where will this pc_next be relevant now? Likely when looping I think. *)
-    (* do pc_next <- trywith "no fallthrough instruction" (incr_pc CFG pc) ;; *)
-    (* match (pt pc), insn  with *)
-
-(* YZ : How should we do handle phi nodes?
-       Seems like option 4 is the way to go.
-       OPTION 1:
-       [| block|]: (block_id * block_id) -> itreeE (block_id * block_id)
-       i.e. We treat elementary blocks as having several entry point, one per
-       adress from which we jumped into it.
-       OPTION 2:
-       We actually perform the semantics of phi nodes at the end of the denotation
-       of the jumping block.
-       i.e. : if b1 := jmp b2 and b2 := x = phi (b1,1; b3,3)
-       then [b1] = send (LocalWrite x 1);; ret b2
-       and of course we do not denote phi nodes first when denoting blocks.
-       Issue (?) Doesn't it break modularity? Can we still loop to tie those things
-       together?
-       OPTION 3:
-       Could the semantics of the phi node use a special event asking the environment
-       where it comes from, and the semantics of the ret using a special event telling
-       the world it's jumping?
-       That kinda implies that now we have two level of handling the control flow of a
-       single function, but avoids both ugly pairs and is completely modular.
-       OPTION 4:
-       Actually, it might be in the function provided to [loop] when denoting
-       a collection of blocks that this should take place so that there is no
-       need for a new effect, it's just that the jmp one does more work.
-     *)
-(*
-      match (find_function_entry CFG fid) with
-      | Some fnentry =>
-        let 'FunctionEntry ids pc_f := fnentry in
-        bs <- combine_lists_err ids dvs ;;
-        let env := env_of_assoc bs in
-        match pt with
-        | IVoid _ =>
-          (debug "pushed void stack frame") ;;
-          cont (g, pc_f, env, (KRet_void e pc_next::k))
-        | IId id =>
-          (debug "pushed non-void stack frame") ;;
-          cont (g, pc_f, env, (KRet e id pc_next::k))
-        end
-      | None =>
-        (* This must have been a registered external function  *)
-        (* We _don't_ push a itree stack frame, since the external *)
-        (* call takes place in one "atomic" step. *)
-
-        match fid with
-        | Name s =>
-          match pt with
-          | IVoid _ =>  (* void externals don't return a value *)
-            vis (Call (eval_typ t) s dvs) (fun dv => cont (g, pc_next, e, k))
-
-                   | IId id => (* non-void externals are assumed to be type correct and bind a value *)
-                     vis (Call (eval_typ t) s dvs)
-                         (fun dv => cont (g, pc_next, add_env id dv e, k))
-                   end
-                 | _ => raise ("step: no function " (* ++ (string_of fid) *))
-                 end
-      end
-       *)
