src/coq/Handlers/Local.v
@@ -2,11 +2,10 @@ From Coq Require Import
      String.
 
 From ExtLib Require Import
-     Programming.Show
      Structures.Monads
      Structures.Maps.
 
-From ITree Require Import 
+From ITree Require Import
      ITree
      Events.State.
 
@@ -17,6 +16,8 @@ From Vellvm Require Import
      DynamicValues
      LLVMEvents
      Error.
+
+Require Import Ceres.Ceres.
 
 Set Implicit Arguments.
 Set Contextual Implicit.
@@ -29,7 +30,7 @@ Section Locals.
   Variable (k v:Type).
   Context {map : Type}.
   Context {M: Map k v map}.
-  Context {SK : Show k}.
+  Context {SK : Serialize k}.
   Definition handle_local {E} `{FailureE -< E} : (LocalE k v) ~> stateT map (itree E) :=
       fun _ e env =>
         match e with
@@ -58,4 +59,3 @@ Section Locals.
     End PARAMS.
 
 End Locals.
-
